src/Lean/Meta/Tactic/Grind/Attr.lean
@@ -63,40 +63,89 @@ def getAttrKindFromOpt (stx : Syntax) : CoreM AttrKind := do
 def throwInvalidUsrModifier : CoreM α :=
   throwError "the modifier `usr` is only relevant in parameters for `grind only`"
 
+private def Extension.addCasesAttr (ext : Extension) (declName : Name) (eager : Bool) (attrKind : AttributeKind) : CoreM Unit := do
+  validateCasesAttr declName eager
+  ext.add (.cases declName eager) attrKind
+
+private def Extension.addExtAttr (ext : Extension) (declName : Name) (attrKind : AttributeKind) : CoreM Unit := do
+  validateExtAttr declName
+  ext.add (.ext declName) attrKind
+
+private def Extension.addFunCCAttr (ext : Extension) (declName : Name) (attrKind : AttributeKind) : CoreM Unit := do
+  ext.add (.funCC declName) attrKind
+
+private def Extension.eraseExtAttr (ext : Extension) (declName : Name) : CoreM Unit := do
+  let s := ext.getState (← getEnv)
+  let extThms ← s.extThms.eraseDecl declName
+  modifyEnv fun env => ext.modifyState env fun s => { s with extThms }
+
+private def Extension.eraseCasesAttr (ext : Extension) (declName : Name) : CoreM Unit := do
+  ensureNotBuiltinCases declName
+  let s := ext.getState (← getEnv)
+  let casesTypes ← s.casesTypes.eraseDecl declName
+  modifyEnv fun env => ext.modifyState env fun s => { s with casesTypes }
+
+private def Extension.eraseFunCCAttr (ext : Extension) (declName : Name) : CoreM Unit := do
+  let s := ext.getState (← getEnv)
+  unless s.funCC.contains declName do
+    throwNotMarkedWithGrindAttribute declName
+  let funCC := s.funCC.erase declName
+  modifyEnv fun env => ext.modifyState env fun s => { s with funCC }
+
+private def Extension.eraseEMatchAttr (ext : Extension) (declName : Name) : MetaM Unit := do
+  let s := ext.getState (← getEnv)
+  let ematch ← s.ematch.eraseDecl declName
+  modifyEnv fun env => ext.modifyState env fun s => { s with ematch }
+
+private def Extension.eraseInjectiveAttr (ext : Extension) (declName : Name) : MetaM Unit := do
+  let s := ext.getState (← getEnv)
+  let inj ← s.inj.eraseDecl declName
+  modifyEnv fun env => ext.modifyState env fun s => { s with inj }
+
+private def Extension.isExtTheorem (ext : Extension) (declName : Name) : CoreM Bool := do
+  return ext.getState (← getEnv) |>.extThms.contains declName
+
+private def Extension.isInjectiveTheorem (ext : Extension) (declName : Name) : CoreM Bool := do
+  return ext.getState (← getEnv) |>.inj.contains (.decl declName)
+
+private def Extension.hasFunCCAttr (ext : Extension) (declName : Name) : CoreM Bool := do
+  return ext.getState (← getEnv) |>.funCC.contains declName
+
 /--
 Auxiliary function for registering `grind`, `grind!`, `grind?`, and `grind!?` attributes.
 `grind!` is like `grind` but selects minimal indexable subterms.
 The `grind?` and `grind!?` are aliases for `grind` and `grind!` which displays patterns using `logInfo`.
 It is just a convenience for users.
 -/
-private def registerGrindAttr (minIndexable : Bool) (showInfo : Bool) : IO Unit :=
+private def mkGrindAttr (attrName : Name) (minIndexable : Bool) (showInfo : Bool) (ext? : Option Extension := none) (ref : Name := by exact decl_name%) : IO Unit :=
   registerBuiltinAttribute {
+    ref  := ref
     name := match minIndexable, showInfo with
-      | false, false => `grind
-      | false, true  => `grind?
-      | true,  false => `grind!
-      | true,  true  => `grind!?
+      | false, false => attrName
+      | false, true  => attrName.appendAfter "?"
+      | true,  false => attrName.appendAfter "!"
+      | true,  true  => attrName.appendAfter "!?"
     descr :=
       let header := match minIndexable, showInfo with
-        | false, false => "The `[grind]` attribute is used to annotate declarations."
-        | false, true  => "The `[grind?]` attribute is identical to the `[grind]` attribute, but displays inferred pattern information."
-        | true,  false => "The `[grind!]` attribute is used to annotate declarations, but selecting minimal indexable subterms."
-        | true,  true  => "The `[grind!?]` attribute is identical to the `[grind!]` attribute, but displays inferred pattern information."
-      header ++ "\
+        | false, false => s!"The `[{attrName}]` attribute is used to annotate declarations."
+        | false, true  => s!"The `[{attrName}?]` attribute is identical to the `[{attrName}]` attribute, but displays inferred pattern information."
+        | true,  false => s!"The `[{attrName}!]` attribute is used to annotate declarations, but selecting minimal indexable subterms."
+        | true,  true  => s!"The `[{attrName}!?]` attribute is identical to the `[{attrName}!]` attribute, but displays inferred pattern information."
+      header ++ s!"\
       \
-      When applied to an equational theorem, `[grind =]`, `[grind =_]`, or `[grind _=_]`\
-      will mark the theorem for use in heuristic instantiations by the `grind` tactic,
+      When applied to an equational theorem, `[{attrName} =]`, `[{attrName} =_]`, or `[{attrName} _=_]`\
+      will mark the theorem for use in heuristic instantiations by the `{attrName}` tactic,
       using respectively the left-hand side, the right-hand side, or both sides of the theorem.\
-      When applied to a function, `[grind =]` automatically annotates the equational theorems associated with that function.\
-      When applied to a theorem `[grind ←]` will instantiate the theorem whenever it encounters the conclusion of the theorem
+      When applied to a function, `[{attrName} =]` automatically annotates the equational theorems associated with that function.\
+      When applied to a theorem `[{attrName} ←]` will instantiate the theorem whenever it encounters the conclusion of the theorem
       (that is, it will use the theorem for backwards reasoning).\
-      When applied to a theorem `[grind →]` will instantiate the theorem whenever it encounters sufficiently many of the propositional hypotheses
+      When applied to a theorem `[{attrName} →]` will instantiate the theorem whenever it encounters sufficiently many of the propositional hypotheses
       (that is, it will use the theorem for forwards reasoning).\
       \
-      The attribute `[grind]` by itself will effectively try `[grind ←]` (if the conclusion is sufficient for instantiation) and then `[grind →]`.\
+      The attribute `[{attrName}]` by itself will effectively try `[{attrName} ←]` (if the conclusion is sufficient for instantiation) and then `[{attrName} →]`.\
       \
       The `grind` tactic utilizes annotated theorems to add instances of matching patterns into the local context during proof search.\
-      For example, if a theorem `@[grind =] theorem foo_idempotent : foo (foo x) = foo x` is annotated,\
+      For example, if a theorem `@[{attrName} =] theorem foo_idempotent : foo (foo x) = foo x` is annotated,\
       `grind` will add an instance of this theorem to the local context whenever it encounters the pattern `foo (foo x)`."
     applicationTime := .afterCompilation
     add := fun declName stx attrKind => MetaM.run' do
@@ -105,49 +154,111 @@ private def registerGrindAttr (minIndexable : Bool) (showInfo : Bool) : IO Unit 
       -- When the body is not available (i.e. the def equations are private), the attribute will not
       -- be exported; see `ematchTheoremsExt.exportEntry?`.
       withoutExporting do
-      match (← getAttrKindFromOpt stx) with
-      | .ematch .user => throwInvalidUsrModifier
-      | .ematch k => addEMatchAttr declName attrKind k (← getGlobalSymbolPriorities) (minIndexable := minIndexable) (showInfo := showInfo)
-      | .cases eager => addCasesAttr declName eager attrKind
-      | .intro =>
-        if let some info ← isCasesAttrPredicateCandidate? declName false then
-          for ctor in info.ctors do
-            addEMatchAttr ctor attrKind (.default false) (← getGlobalSymbolPriorities) (minIndexable := minIndexable) (showInfo := showInfo)
-        else
-          throwError "invalid `[grind intro]`, `{.ofConstName declName}` is not an inductive predicate"
-      | .ext => addExtAttr declName attrKind
-      | .infer =>
-        if let some declName ← isCasesAttrCandidate? declName false then
-          addCasesAttr declName false attrKind
-          if let some info ← isInductivePredicate? declName then
-            -- If it is an inductive predicate,
-            -- we also add the constructors (intro rules) as E-matching rules
+      if let some ext := ext? then
+        match (← getAttrKindFromOpt stx) with
+        | .symbol prio =>
+          unless attrName == `grind do
+            throwError "symbol priorities must be set using the default `[grind]` attribute"
+          addSymbolPriorityAttr declName attrKind prio
+        | .cases eager => ext.addCasesAttr declName eager attrKind
+        | .funCC => ext.addFunCCAttr declName attrKind
+        | .ext => ext.addExtAttr declName attrKind
+        | .ematch .user => throwInvalidUsrModifier
+        | .ematch k => ext.addEMatchAttr declName attrKind k (← getGlobalSymbolPriorities) (minIndexable := minIndexable) (showInfo := showInfo)
+        | .intro =>
+          if let some info ← isCasesAttrPredicateCandidate? declName false then
+            for ctor in info.ctors do
+              ext.addEMatchAttr ctor attrKind (.default false) (← getGlobalSymbolPriorities) (minIndexable := minIndexable) (showInfo := showInfo)
+          else
+            throwError "invalid `[{attrName} intro]`, `{.ofConstName declName}` is not an inductive predicate"
+        | .infer =>
+          if let some declName ← isCasesAttrCandidate? declName false then
+            ext.addCasesAttr declName false attrKind
+            if let some info ← isInductivePredicate? declName then
+              -- If it is an inductive predicate,
+              -- we also add the constructors (intro rules) as E-matching rules
+              for ctor in info.ctors do
+                ext.addEMatchAttr ctor attrKind (.default false) (← getGlobalSymbolPriorities) (minIndexable := minIndexable) (showInfo := showInfo)
+          else
+            ext.addEMatchAttrAndSuggest stx declName attrKind (← getGlobalSymbolPriorities) (minIndexable := minIndexable) (showInfo := showInfo)
+        | .inj => ext.addInjectiveAttr declName attrKind
+      else
+        -- **TODO**: delete after update stage0 and new extension for default `grind` attribute
+        match (← getAttrKindFromOpt stx) with
+        | .ematch .user => throwInvalidUsrModifier
+        | .ematch k => addEMatchAttr declName attrKind k (← getGlobalSymbolPriorities) (minIndexable := minIndexable) (showInfo := showInfo)
+        | .cases eager => addCasesAttr declName eager attrKind
+        | .intro =>
+          if let some info ← isCasesAttrPredicateCandidate? declName false then
             for ctor in info.ctors do
               addEMatchAttr ctor attrKind (.default false) (← getGlobalSymbolPriorities) (minIndexable := minIndexable) (showInfo := showInfo)
-        else
-          addEMatchAttrAndSuggest stx declName attrKind (← getGlobalSymbolPriorities) (minIndexable := minIndexable) (showInfo := showInfo)
-      | .symbol prio => addSymbolPriorityAttr declName attrKind prio
-      | .inj => addInjectiveAttr declName attrKind
-      | .funCC => addFunCCAttr declName attrKind
+          else
+            throwError "invalid `[{attrName} intro]`, `{.ofConstName declName}` is not an inductive predicate"
+        | .ext => addExtAttr declName attrKind
+        | .infer =>
+          if let some declName ← isCasesAttrCandidate? declName false then
+            addCasesAttr declName false attrKind
+            if let some info ← isInductivePredicate? declName then
+              -- If it is an inductive predicate,
+              -- we also add the constructors (intro rules) as E-matching rules
+              for ctor in info.ctors do
+                addEMatchAttr ctor attrKind (.default false) (← getGlobalSymbolPriorities) (minIndexable := minIndexable) (showInfo := showInfo)
+          else
+            addEMatchAttrAndSuggest stx declName attrKind (← getGlobalSymbolPriorities) (minIndexable := minIndexable) (showInfo := showInfo)
+        | .symbol prio => addSymbolPriorityAttr declName attrKind prio
+        | .inj => addInjectiveAttr declName attrKind
+        | .funCC => addFunCCAttr declName attrKind
     erase := fun declName => MetaM.run' do
       if showInfo then
-        throwError "`[grind?]` is a helper attribute for displaying inferred patterns, if you want to remove the attribute, consider using `[grind]` instead"
-      if (← isCasesAttrCandidate declName false) then
-        eraseCasesAttr declName
-      else if (← isExtTheorem declName) then
-        eraseExtAttr declName
-      else if (← isInjectiveTheorem declName) then
-        eraseInjectiveAttr declName
-      else if (← hasFunCCAttr declName) then
-        eraseFunCCAttr declName
+        throwError "`[{attrName}?]` is a helper attribute for displaying inferred patterns, if you want to remove the attribute, consider using `[{attrName}]` instead"
+      if let some ext := ext? then
+        if (← isCasesAttrCandidate declName false) then
+          ext.eraseCasesAttr declName
+        else if (← ext.isExtTheorem declName) then
+          ext.eraseExtAttr declName
+        else if (← ext.isInjectiveTheorem declName) then
+          ext.eraseInjectiveAttr declName
+        else if (← ext.hasFunCCAttr declName) then
+          ext.eraseFunCCAttr declName
+        else
+          ext.eraseEMatchAttr declName
       else
-        eraseEMatchAttr declName
+        -- **TODO**: delete after update stage0 and new extension for default `grind` attribute
+        if (← isCasesAttrCandidate declName false) then
+          eraseCasesAttr declName
+        else if (← isExtTheorem declName) then
+          eraseExtAttr declName
+        else if (← isInjectiveTheorem declName) then
+          eraseInjectiveAttr declName
+        else if (← hasFunCCAttr declName) then
+          eraseFunCCAttr declName
+        else
+          eraseEMatchAttr declName
   }
 
+private def registerDefaultGrindAttr (minIndexable : Bool) (showInfo : Bool) : IO Unit :=
+  mkGrindAttr `grind minIndexable showInfo
+
 builtin_initialize
-  registerGrindAttr (minIndexable := false) (showInfo := true)
-  registerGrindAttr (minIndexable := false) (showInfo := false)
-  registerGrindAttr (minIndexable := true) (showInfo := true)
-  registerGrindAttr (minIndexable := true) (showInfo := false)
+  registerDefaultGrindAttr (minIndexable := false) (showInfo := true)
+  registerDefaultGrindAttr (minIndexable := false) (showInfo := false)
+  registerDefaultGrindAttr (minIndexable := true) (showInfo := true)
+  registerDefaultGrindAttr (minIndexable := true) (showInfo := false)
+
+abbrev ExtensionMap := Std.HashMap Name Extension
+
+builtin_initialize extensionMapRef : IO.Ref ExtensionMap ← IO.mkRef {}
+
+def getExtension? (attrName : Name) : IO (Option Extension) :=
+  return (← extensionMapRef.get)[attrName]?
+
+def registerAttr (attrName : Name) (ref : Name := by exact decl_name%) : IO Extension := do
+  let ext ← mkExtension ref
+  mkGrindAttr attrName (minIndexable := false) (showInfo := true) (ext? := some ext) (ref := ref)
+  mkGrindAttr attrName (minIndexable := false) (showInfo := false) (ext? := some ext) (ref := ref)
+  mkGrindAttr attrName (minIndexable := true) (showInfo := true) (ext? := some ext) (ref := ref)
+  mkGrindAttr attrName (minIndexable := true) (showInfo := false) (ext? := some ext) (ref := ref)
+  extensionMapRef.modify fun map => map.insert attrName ext
+  return ext
 
 end Lean.Meta.Grind
