src/Lean/Meta/Tactic/Grind/Cases.lean
@@ -6,18 +6,17 @@ Authors: Leonardo de Moura
 module
 prelude
 public import Lean.Meta.Tactic.Cases
+public import Lean.Meta.Tactic.Grind.Extension
 public section
 namespace Lean.Meta.Grind
-
-/-- Types that `grind` will case-split on. -/
-structure CasesTypes where
-  casesMap : PHashMap Name Bool := {}
-  deriving Inhabited
-
+-- TODO: delete
 structure CasesEntry where
   declName : Name
   eager : Bool
   deriving Inhabited
+
+/-- A collection of `CasesTypes`. -/
+abbrev CasesTypesArray := Array CasesTypes
 
 /--
 `grind` always case-splits on the following types. Even when using `grind only`.
@@ -43,9 +42,6 @@ def CasesTypes.contains (s : CasesTypes) (declName : Name) : Bool :=
 def CasesTypes.erase (s : CasesTypes) (declName : Name) : CasesTypes :=
   { s with casesMap := s.casesMap.erase declName }
 
-def CasesTypes.insert (s : CasesTypes) (declName : Name) (eager : Bool) : CasesTypes :=
-  { s with casesMap := s.casesMap.insert declName eager }
-
 def CasesTypes.find? (s : CasesTypes) (declName : Name) : Option Bool :=
   s.casesMap.find? declName
 
@@ -55,6 +51,9 @@ def CasesTypes.isEagerSplit (s : CasesTypes) (declName : Name) : Bool :=
 def CasesTypes.isSplit (s : CasesTypes) (declName : Name) : Bool :=
   (s.casesMap.find? declName |>.isSome) || isBuiltinEagerCases declName
 
+/-
+TODO: group into a `grind` extension object
+-/
 builtin_initialize casesExt : SimpleScopedEnvExtension CasesEntry CasesTypes ←
   registerSimpleScopedEnvExtension {
     initial        := {}
@@ -68,7 +67,7 @@ def getCasesTypes : CoreM CasesTypes :=
   return casesExt.getState (← getEnv)
 
 /-- Returns `true` is `declName` is a builtin split or has been tagged with `[grind]` attribute. -/
-def isSplit (declName : Name) : CoreM Bool := do
+def isGlobalSplit (declName : Name) : CoreM Bool := do
   return (← getCasesTypes).isSplit declName
 
 partial def isCasesAttrCandidate? (declName : Name) (eager : Bool) : CoreM (Option Name) := do
@@ -98,7 +97,7 @@ def CasesTypes.eraseDecl (s : CasesTypes) (declName : Name) : CoreM CasesTypes :
   if s.contains declName then
     return s.erase declName
   else
-    throwError "`{.ofConstName declName}` is not marked with the `[grind]` attribute"
+    throwNotMarkedWithGrindAttribute declName
 
 def ensureNotBuiltinCases (declName : Name) : CoreM Unit := do
   if isBuiltinEagerCases declName then
