src/Lean/Meta/Tactic/Grind/ExtAttr.lean
@@ -6,13 +6,14 @@ Authors: Leonardo de Moura
 module
 prelude
 public import Lean.Meta.Tactic.Ext
+public import Lean.Meta.Tactic.Grind.Extension
 public section
 namespace Lean.Meta.Grind
 /-! Grind extensionality attribute to mark which `[ext]` theorems should be used. -/
 
-/-- Extensionality theorems that can be used by `grind` -/
-abbrev ExtTheorems := PHashSet Name
-
+/-
+TODO: group into a `grind` extension object
+-/
 builtin_initialize extTheoremsExt : SimpleScopedEnvExtension Name ExtTheorems ←
   registerSimpleScopedEnvExtension {
     initial        := {}
@@ -28,7 +29,7 @@ def addExtAttr (declName : Name) (attrKind : AttributeKind) : CoreM Unit := do
   validateExtAttr declName
   extTheoremsExt.add declName attrKind
 
-private def eraseDecl (s : ExtTheorems) (declName : Name) : CoreM ExtTheorems := do
+def ExtTheorems.eraseDecl (s : ExtTheorems) (declName : Name) : CoreM ExtTheorems := do
   if s.contains declName then
     return s.erase declName
   else
@@ -36,10 +37,13 @@ private def eraseDecl (s : ExtTheorems) (declName : Name) : CoreM ExtTheorems :=
 
 def eraseExtAttr (declName : Name) : CoreM Unit := do
   let s := extTheoremsExt.getState (← getEnv)
-  let s ← eraseDecl s declName
+  let s ← s.eraseDecl declName
   modifyEnv fun env => extTheoremsExt.modifyState env fun _ => s
 
 def isExtTheorem (declName : Name) : CoreM Bool := do
   return extTheoremsExt.getState (← getEnv) |>.contains declName
+
+def getGlobalExtTheorems : CoreM ExtTheorems := do
+  return extTheoremsExt.getState (← getEnv)
 
 end Lean.Meta.Grind
