src/Lean/Meta/Tactic/Grind/RegisterCommand.lean
@@ -1,0 +1,30 @@
+/-
+Copyright (c) 2025 Amazon.com, Inc. or its affiliates. All Rights Reserved.
+Released under Apache 2.0 license as described in the file LICENSE.
+Authors: Leonardo de Moura
+-/
+module
+prelude
+public import Lean.Meta.Tactic.Grind.Types
+meta import Lean.Meta.Tactic.Grind.Attr
+public section
+namespace Lean.Meta.Grind
+
+macro (name := _root_.Lean.Parser.Command.registerGrindAttr) doc:(docComment)?
+  "register_grind_attr" id:ident : command => do
+  let str1 := id.getId.toString
+  let idParser1 := mkIdentFrom id (`Lean.Parser.Attr ++ id.getId)
+  let str2 := id.getId.toString ++ "!"
+  let idParser2 := mkIdentFrom id (`Lean.Parser.Attr ++ (id.getId.appendAfter "!"))
+  let str3 := id.getId.toString ++ "?"
+  let idParser3 := mkIdentFrom id (`Lean.Parser.Attr ++ (id.getId.appendAfter "?"))
+  let str4 := id.getId.toString ++ "!?"
+  let idParser4 := mkIdentFrom id (`Lean.Parser.Attr ++ (id.getId.appendAfter "!?"))
+  `($[$doc:docComment]? initialize ext : Extension ← registerAttr $(quote id.getId) (ref := $(quote id.getId))
+    $[$doc:docComment]? syntax (name := $idParser1:ident) $(quote str1):str (ppSpace Lean.Parser.Attr.grindMod)? : attr
+    $[$doc:docComment]? syntax (name := $idParser2:ident) $(quote str2):str (ppSpace Lean.Parser.Attr.grindMod)? : attr
+    $[$doc:docComment]? syntax (name := $idParser3:ident) $(quote str3):str (ppSpace Lean.Parser.Attr.grindMod)? : attr
+    $[$doc:docComment]? syntax (name := $idParser4:ident) $(quote str4):str (ppSpace Lean.Parser.Attr.grindMod)? : attr
+    )
+
+end Lean.Meta.Grind
