src/Lean/Meta/Tactic/Grind/SimpUtil.lean
@@ -18,6 +18,9 @@ import Init.Grind.Norm
 public section
 namespace Lean.Meta.Grind
 
+/-
+TODO: group into a `grind` extension object
+-/
 builtin_initialize normExt : SimpExtension ← mkSimpExt
 
 def registerNormTheorems (preDeclNames : Array Name) (postDeclNames : Array Name) : MetaM Unit := do
@@ -176,14 +179,18 @@ private def addDeclToUnfold (s : SimpTheorems) (declName : Name) : MetaM SimpThe
   else
     return s
 
-/-- Returns the simplification context used by `grind`. -/
-protected def getSimpContext (config : Grind.Config) : MetaM Simp.Context := do
+def getNormTheorems : MetaM SimpTheorems := do
   let mut thms ← normExt.getTheorems
   thms ← addDeclToUnfold thms ``GE.ge
   thms ← addDeclToUnfold thms ``GT.gt
   thms ← addDeclToUnfold thms ``Nat.cast
   thms ← addDeclToUnfold thms ``Bool.xor
   thms ← addDeclToUnfold thms ``Ne
+  return thms
+
+/-- Returns the simplification context used by `grind`. -/
+protected def getSimpContext (config : Grind.Config) : MetaM Simp.Context := do
+  let thms ← getNormTheorems
   Simp.mkContext
     (config :=
       { arith := true
